Examples/UniswapV2Pair/Routines.lean
@@ -1093,8 +1093,7 @@ theorem uniswapTransferLogMem_size (src toWord value : UInt256) :
   rw [toByteArray_write_eq _ _ _ (by rw [uniswapTransferCreditHashMem_size]; omega)
       (by rw [uniswapTransferCreditHashMem_size]; exact lt_usize _ (by norm_num)),
     ByteArray.size_append, ByteArray.size_append, uniswapTransferCreditHashMem_size,
-    ByteArray_zeroes_size,
-    USize.toNat_ofNat_of_lt' (lt_usize _ (by norm_num)), toByteArray_size]
+    ByteArray_zeroes_size, toByteArray_size]
 
 theorem uniswapTransferLogMem_read64 (src toWord value : UInt256) :
     (uniswapTransferLogMem src toWord value).readWithPadding 64 32 =
@@ -1108,7 +1107,6 @@ theorem uniswapTransferLogMem_read64 (src toWord value : UInt256) :
       native_decide)]
   rw [extract_append_left _ _ _ _ (by
       rw [ByteArray.size_append, uniswapTransferCreditHashMem_size, ByteArray_zeroes_size]
-      rw [USize.toNat_ofNat_of_lt' (lt_usize _ (by norm_num))]
       omega)]
   rw [extract_append_left _ _ _ _ (by rw [uniswapTransferCreditHashMem_size]),
     ← readWithPadding_eq_extract _ 64 (by rw [uniswapTransferCreditHashMem_size]),
@@ -1133,17 +1131,13 @@ theorem uniswapTransferLogMem_read128 (src toWord value : UInt256) :
       (by rw [uniswapTransferCreditHashMem_size]; exact lt_usize _ (by norm_num))]
   rw [readWithPadding_eq_extract _ 128 (by
       rw [ByteArray.size_append, ByteArray.size_append, uniswapTransferCreditHashMem_size,
-        ByteArray_zeroes_size, USize.toNat_ofNat_of_lt' (lt_usize _ (by norm_num)),
-        toByteArray_size])]
+        ByteArray_zeroes_size, toByteArray_size])]
   rw [extract_append_right_window
       (uniswapTransferCreditHashMem src toWord ++
-        ffi.ByteArray.zeroes
-          (USize.ofNat (128 - (uniswapTransferCreditHashMem src toWord).size)))
+        ffi.ByteArray.zeroes (128 - (uniswapTransferCreditHashMem src toWord).size))
       (UInt256.toByteArray value) 128 (128 + 32) (by
-        rw [ByteArray.size_append, uniswapTransferCreditHashMem_size, ByteArray_zeroes_size]
-        rw [USize.toNat_ofNat_of_lt' (lt_usize _ (by norm_num))])]
+        rw [ByteArray.size_append, uniswapTransferCreditHashMem_size, ByteArray_zeroes_size])]
   rw [ByteArray.size_append, uniswapTransferCreditHashMem_size, ByteArray_zeroes_size]
-  rw [USize.toNat_ofNat_of_lt' (lt_usize _ (by norm_num))]
   norm_num
   apply ByteArray.ext
   rw [ByteArray.data_extract]
@@ -1356,8 +1350,7 @@ theorem uniswapApproveLogMem_size (owner spender value : UInt256) :
   rw [toByteArray_write_eq _ _ _ (by rw [uniswapApproveHashMem_size]; omega)
       (by rw [uniswapApproveHashMem_size]; exact lt_usize _ (by norm_num)),
     ByteArray.size_append, ByteArray.size_append, uniswapApproveHashMem_size,
-    ByteArray_zeroes_size,
-    USize.toNat_ofNat_of_lt' (lt_usize _ (by norm_num)), toByteArray_size]
+    ByteArray_zeroes_size, toByteArray_size]
 
 theorem uniswapApproveLogMem_read64 (owner spender value : UInt256) :
     (uniswapApproveLogMem owner spender value).readWithPadding 64 32 =
@@ -1371,7 +1364,6 @@ theorem uniswapApproveLogMem_read64 (owner spender value : UInt256) :
       native_decide)]
   rw [extract_append_left _ _ _ _ (by
       rw [ByteArray.size_append, uniswapApproveHashMem_size, ByteArray_zeroes_size]
-      rw [USize.toNat_ofNat_of_lt' (lt_usize _ (by norm_num))]
       omega)]
   rw [extract_append_left _ _ _ _ (by rw [uniswapApproveHashMem_size]),
     ← readWithPadding_eq_extract _ 64 (by rw [uniswapApproveHashMem_size]),
@@ -1396,16 +1388,13 @@ theorem uniswapApproveLogMem_read128 (owner spender value : UInt256) :
       (by rw [uniswapApproveHashMem_size]; exact lt_usize _ (by norm_num))]
   rw [readWithPadding_eq_extract _ 128 (by
       rw [ByteArray.size_append, ByteArray.size_append, uniswapApproveHashMem_size,
-        ByteArray_zeroes_size, USize.toNat_ofNat_of_lt' (lt_usize _ (by norm_num)),
-        toByteArray_size])]
+        ByteArray_zeroes_size, toByteArray_size])]
   rw [extract_append_right_window
       (uniswapApproveHashMem owner spender ++
-        ffi.ByteArray.zeroes (USize.ofNat (128 - (uniswapApproveHashMem owner spender).size)))
+        ffi.ByteArray.zeroes (128 - (uniswapApproveHashMem owner spender).size))
       (UInt256.toByteArray value) 128 (128 + 32) (by
-        rw [ByteArray.size_append, uniswapApproveHashMem_size, ByteArray_zeroes_size]
-        rw [USize.toNat_ofNat_of_lt' (lt_usize _ (by norm_num))])]
+        rw [ByteArray.size_append, uniswapApproveHashMem_size, ByteArray_zeroes_size])]
   rw [ByteArray.size_append, uniswapApproveHashMem_size, ByteArray_zeroes_size]
-  rw [USize.toNat_ofNat_of_lt' (lt_usize _ (by norm_num))]
   norm_num
   apply ByteArray.ext
   rw [ByteArray.data_extract]
